<?xml version="1.0"?>
<rdf:RDF xmlns="http://example.org/OntologiaTurismo#"
     xml:base="http://example.org/OntologiaTurismo"
     xmlns:owl="http://www.w3.org/2002/07/owl#"
     xmlns:rdf="http://www.w3.org/1999/02/22-rdf-syntax-ns#"
     xmlns:xml="http://www.w3.org/XML/1998/namespace"
     xmlns:xsd="http://www.w3.org/2001/XMLSchema#"
     xmlns:owl1="http://www.w3.org/2002/07/owl#owl:"
     xmlns:rdfs="http://www.w3.org/2000/01/rdf-schema#"
     xmlns:swrl="http://www.w3.org/2003/11/swrl#"
     xmlns:swrla="http://swrl.stanford.edu/ontologies/3.3/swrla.owl#"
     xmlns:swrlb="http://www.w3.org/2003/11/swrlb#"
     xmlns:terms="http://purl.org/dc/terms/"
     xmlns:turismo="http://www.ejemplo.org/ontologias/turismo#">
    <owl:Ontology rdf:about="http://example.org/OntologiaTurismo">
        <terms:description>An ontology that describes different types of tourist resources in various cities across Spain</terms:description>
        <terms:issued>2025-04-19</terms:issued>
        <terms:modified>2025-04-19</terms:modified>
        <terms:publisher>Alfredo Benítez Vargas, Computer Engineering student at the Universitat Oberta de Catalunya (UOC)</terms:publisher>
        <terms:title>Ontology of Tourism in Spain</terms:title>
    </owl:Ontology>
    


    <!-- 
    ///////////////////////////////////////////////////////////////////////////////////////
    //
    // Annotation properties
    //
    ///////////////////////////////////////////////////////////////////////////////////////
     -->


    


    <!-- http://purl.org/dc/terms/description -->


    <owl:AnnotationProperty rdf:about="http://purl.org/dc/terms/description"/>
    


    <!-- http://purl.org/dc/terms/issued -->


    <owl:AnnotationProperty rdf:about="http://purl.org/dc/terms/issued"/>
    


    <!-- http://purl.org/dc/terms/modified -->


    <owl:AnnotationProperty rdf:about="http://purl.org/dc/terms/modified"/>
    


    <!-- http://purl.org/dc/terms/publisher -->


    <owl:AnnotationProperty rdf:about="http://purl.org/dc/terms/publisher"/>
    


    <!-- http://purl.org/dc/terms/title -->


    <owl:AnnotationProperty rdf:about="http://purl.org/dc/terms/title"/>
    


    <!-- http://swrl.stanford.edu/ontologies/3.3/swrla.owl#isRuleEnabled -->


    <owl:AnnotationProperty rdf:about="http://swrl.stanford.edu/ontologies/3.3/swrla.owl#isRuleEnabled"/>
    


    <!-- http://www.w3.org/2002/07/owl#owl:sameAs -->


    <owl:AnnotationProperty rdf:about="http://www.w3.org/2002/07/owl#owl:sameAs">
        <rdfs:comment>Indicates that two resources refer to the same real-world entity</rdfs:comment>
        <rdfs:label>owl:sameAs</rdfs:label>
    </owl:AnnotationProperty>
    


    <!-- 
    ///////////////////////////////////////////////////////////////////////////////////////
    //
    // Object Properties
    //
    ///////////////////////////////////////////////////////////////////////////////////////
     -->


    


    <!-- http://www.ejemplo.org/ontologias/turismo#HasTypesOfTransportation -->


    <owl:ObjectProperty rdf:about="http://www.ejemplo.org/ontologias/turismo#HasTypesOfTransportation">
        <rdfs:domain rdf:resource="http://www.ejemplo.org/ontologias/turismo#Cities"/>
        <rdfs:range rdf:resource="http://www.ejemplo.org/ontologias/turismo#Transports"/>
        <rdfs:comment>Relates a city to the types of transportation systems available in it</rdfs:comment>
        <rdfs:label>HasTypesOfTransportation</rdfs:label>
    </owl:ObjectProperty>
    


    <!-- http://www.ejemplo.org/ontologias/turismo#HeldIn -->


    <owl:ObjectProperty rdf:about="http://www.ejemplo.org/ontologias/turismo#HeldIn">
        <rdf:type rdf:resource="http://www.w3.org/2002/07/owl#FunctionalProperty"/>
        <rdfs:domain rdf:resource="http://www.ejemplo.org/ontologias/turismo#Events"/>
        <rdfs:range rdf:resource="http://www.ejemplo.org/ontologias/turismo#Cities"/>
        <rdfs:comment>Relates an event to the city where it takes place</rdfs:comment>
        <rdfs:label>HeldIn</rdfs:label>
    </owl:ObjectProperty>
    


    <!-- http://www.ejemplo.org/ontologias/turismo#LocatedIn -->


    <owl:ObjectProperty rdf:about="http://www.ejemplo.org/ontologias/turismo#LocatedIn">
        <rdf:type rdf:resource="http://www.w3.org/2002/07/owl#FunctionalProperty"/>
        <rdfs:domain rdf:resource="http://www.ejemplo.org/ontologias/turismo#Attractions"/>
        <rdfs:range rdf:resource="http://www.ejemplo.org/ontologias/turismo#Cities"/>
        <rdfs:comment>Indicates the city in which a given tourism-related entity, such as an attraction, restaurant, hotel, or event, is located</rdfs:comment>
        <rdfs:label>LocatedIn</rdfs:label>
    </owl:ObjectProperty>
    


    <!-- 
    ///////////////////////////////////////////////////////////////////////////////////////
    //
    // Data properties
    //
    ///////////////////////////////////////////////////////////////////////////////////////
     -->


    


    <!-- http://www.ejemplo.org/ontologias/turismo#hasARating -->


    <owl:DatatypeProperty rdf:about="http://www.ejemplo.org/ontologias/turismo#hasARating">
        <rdf:type rdf:resource="http://www.w3.org/2002/07/owl#FunctionalProperty"/>
        <rdfs:domain rdf:resource="http://www.ejemplo.org/ontologias/turismo#Restaurants"/>
        <rdfs:range rdf:resource="http://www.w3.org/2001/XMLSchema#decimal"/>
        <rdfs:comment>Represents the average rating score of a restaurant as a decimal number</rdfs:comment>
        <rdfs:label>hasARating</rdfs:label>
    </owl:DatatypeProperty>
    


    <!-- http://www.ejemplo.org/ontologias/turismo#hasName -->


    <owl:DatatypeProperty rdf:about="http://www.ejemplo.org/ontologias/turismo#hasName">
        <rdfs:subPropertyOf rdf:resource="http://www.w3.org/2002/07/owl#topDataProperty"/>
        <rdf:type rdf:resource="http://www.w3.org/2002/07/owl#FunctionalProperty"/>
        <rdfs:domain rdf:resource="http://www.ejemplo.org/ontologias/turismo#Hotels"/>
        <rdfs:range rdf:resource="http://www.w3.org/2001/XMLSchema#string"/>
        <rdfs:comment>Represents the official name of a hotel as a text string</rdfs:comment>
        <rdfs:label>hasName</rdfs:label>
    </owl:DatatypeProperty>
    


    <!-- 
    ///////////////////////////////////////////////////////////////////////////////////////
    //
    // Classes
    //
    ///////////////////////////////////////////////////////////////////////////////////////
     -->


    


    <!-- http://www.ejemplo.org/ontologias/turismo#AmusementPark -->


    <owl:Class rdf:about="http://www.ejemplo.org/ontologias/turismo#AmusementPark">
        <rdfs:subClassOf rdf:resource="http://www.ejemplo.org/ontologias/turismo#Attractions"/>
        <rdfs:comment>A recreational area with various rides, games, and entertainment, designed for family fun and leisure</rdfs:comment>
        <rdfs:label>AmusementPark</rdfs:label>
    </owl:Class>
    


    <!-- http://www.ejemplo.org/ontologias/turismo#Andalusian -->


    <owl:Class rdf:about="http://www.ejemplo.org/ontologias/turismo#Andalusian">
        <rdfs:subClassOf rdf:resource="http://www.ejemplo.org/ontologias/turismo#Restaurants"/>
        <rdfs:comment>Establishments that serve traditional Andalusian cuisine, known for its Mediterranean flavors, use of olive oil, and regional specialties like gazpacho and pescaíto frito</rdfs:comment>
        <rdfs:label>Andalusian</rdfs:label>
    </owl:Class>
    


    <!-- http://www.ejemplo.org/ontologias/turismo#Attractions -->


    <owl:Class rdf:about="http://www.ejemplo.org/ontologias/turismo#Attractions">
        <rdfs:subClassOf rdf:resource="http://www.ejemplo.org/ontologias/turismo#Tourism"/>
        <rdfs:comment>Attractions are places or activities of interest that draw tourists, such as landmarks, natural wonders, museums, or amusement parks</rdfs:comment>
        <rdfs:label>Attractions</rdfs:label>
    </owl:Class>
    


    <!-- http://www.ejemplo.org/ontologias/turismo#BeachAttraction -->


    <owl:Class rdf:about="http://www.ejemplo.org/ontologias/turismo#BeachAttraction">
        <rdfs:subClassOf rdf:resource="http://www.ejemplo.org/ontologias/turismo#Attractions"/>
        <rdfs:comment>A coastal location or area, typically known for its natural beauty, offering recreational activities such as swimming, sunbathing, and beach sports</rdfs:comment>
        <rdfs:label>BeachAttraction</rdfs:label>
    </owl:Class>
    


    <!-- http://www.ejemplo.org/ontologias/turismo#BeachHotel -->


    <owl:Class rdf:about="http://www.ejemplo.org/ontologias/turismo#BeachHotel">
        <rdfs:subClassOf rdf:resource="http://www.ejemplo.org/ontologias/turismo#Hotels"/>
        <rdfs:comment>Hotels located near or on the beach, offering easy access to the coastline and beach-related amenities</rdfs:comment>
        <rdfs:label>BeachHotel</rdfs:label>
    </owl:Class>
    


    <!-- http://www.ejemplo.org/ontologias/turismo#Bicycle -->


    <owl:Class rdf:about="http://www.ejemplo.org/ontologias/turismo#Bicycle">
        <rdfs:subClassOf rdf:resource="http://www.ejemplo.org/ontologias/turismo#Transports"/>
        <rdfs:comment>Bicycle is a human-powered transport vehicle with two wheels, commonly used for short-distance travel and recreational purposes</rdfs:comment>
        <rdfs:label>Bicycle</rdfs:label>
    </owl:Class>
    


    <!-- http://www.ejemplo.org/ontologias/turismo#BigCity -->


    <owl:Class rdf:about="http://www.ejemplo.org/ontologias/turismo#BigCity">
        <rdfs:subClassOf rdf:resource="http://www.ejemplo.org/ontologias/turismo#Cities"/>
        <rdfs:comment>Represents a city that has metro transportation and is classified as a big city</rdfs:comment>
        <rdfs:label>BigCity</rdfs:label>
    </owl:Class>
    


    <!-- http://www.ejemplo.org/ontologias/turismo#Bus -->


    <owl:Class rdf:about="http://www.ejemplo.org/ontologias/turismo#Bus">
        <rdfs:subClassOf rdf:resource="http://www.ejemplo.org/ontologias/turismo#Transports"/>
        <rdfs:comment>Bus is a type of public transport that operates on fixed routes and schedules, commonly used for travel within and between cities</rdfs:comment>
        <rdfs:label>Bus</rdfs:label>
    </owl:Class>
    


    <!-- http://www.ejemplo.org/ontologias/turismo#Business -->


    <owl:Class rdf:about="http://www.ejemplo.org/ontologias/turismo#Business">
        <rdfs:subClassOf rdf:resource="http://www.ejemplo.org/ontologias/turismo#Hotels"/>
        <rdfs:comment>Hotels that cater primarily to business travelers, providing amenities such as conference rooms, workspaces, and high-speed internet</rdfs:comment>
        <rdfs:label>Business</rdfs:label>
    </owl:Class>
    


    <!-- http://www.ejemplo.org/ontologias/turismo#Cities -->


    <owl:Class rdf:about="http://www.ejemplo.org/ontologias/turismo#Cities">
        <rdfs:subClassOf rdf:resource="http://www.ejemplo.org/ontologias/turismo#Tourism"/>
        <rdfs:comment>Cities are large human settlements that often serve as central destinations for tourism due to their cultural, historical, or economic significance</rdfs:comment>
        <rdfs:label>Cities</rdfs:label>
    </owl:Class>
    


    <!-- http://www.ejemplo.org/ontologias/turismo#CityWithEvents -->


    <owl:Class rdf:about="http://www.ejemplo.org/ontologias/turismo#CityWithEvents">
        <rdfs:subClassOf rdf:resource="http://www.ejemplo.org/ontologias/turismo#Cities"/>
        <rdfs:comment>Represents a city that hosts at least one event</rdfs:comment>
        <rdfs:label>CityWithEvents</rdfs:label>
    </owl:Class>
    


    <!-- http://www.ejemplo.org/ontologias/turismo#CulturalAttraction -->


    <owl:Class rdf:about="http://www.ejemplo.org/ontologias/turismo#CulturalAttraction">
        <rdfs:subClassOf rdf:resource="http://www.ejemplo.org/ontologias/turismo#Attractions"/>
        <rdfs:comment>Attractions that highlight the cultural heritage of a region, such as museums, historical sites, theaters, and art galleries</rdfs:comment>
        <rdfs:label>CulturalAttractions</rdfs:label>
    </owl:Class>
    


    <!-- http://www.ejemplo.org/ontologias/turismo#CulturalCity -->


    <owl:Class rdf:about="http://www.ejemplo.org/ontologias/turismo#CulturalCity">
        <rdfs:subClassOf rdf:resource="http://www.ejemplo.org/ontologias/turismo#Cities"/>
        <rdfs:comment>City with cultural events</rdfs:comment>
        <rdfs:label>CulturalCity</rdfs:label>
    </owl:Class>
    


    <!-- http://www.ejemplo.org/ontologias/turismo#CulturalEvent -->


    <owl:Class rdf:about="http://www.ejemplo.org/ontologias/turismo#CulturalEvent">
        <rdfs:subClassOf rdf:resource="http://www.ejemplo.org/ontologias/turismo#Events"/>
        <rdfs:comment>Events that celebrate and showcase cultural activities, such as theater performances, art exhibitions, and traditional festivals</rdfs:comment>
        <rdfs:label>CulturalEvent</rdfs:label>
    </owl:Class>
    


    <!-- http://www.ejemplo.org/ontologias/turismo#Events -->


    <owl:Class rdf:about="http://www.ejemplo.org/ontologias/turismo#Events">
        <rdfs:subClassOf rdf:resource="http://www.ejemplo.org/ontologias/turismo#Tourism"/>
        <rdfs:subClassOf>
            <owl:Restriction>
                <owl:onProperty rdf:resource="http://www.ejemplo.org/ontologias/turismo#HeldIn"/>
                <owl:someValuesFrom rdf:resource="http://www.ejemplo.org/ontologias/turismo#Cities"/>
            </owl:Restriction>
        </rdfs:subClassOf>
        <rdfs:comment>Events are organized activities or occurrences intended to attract tourists, such as festivals, exhibitions, or cultural performances</rdfs:comment>
        <rdfs:label>Events</rdfs:label>
    </owl:Class>
    


    <!-- http://www.ejemplo.org/ontologias/turismo#Gastronomic -->


    <owl:Class rdf:about="http://www.ejemplo.org/ontologias/turismo#Gastronomic">
        <rdfs:subClassOf rdf:resource="http://www.ejemplo.org/ontologias/turismo#Events"/>
        <rdfs:comment>Events focused on food and culinary experiences, such as food festivals, cooking classes, and gastronomic tours</rdfs:comment>
        <rdfs:label>Gastronomic</rdfs:label>
    </owl:Class>
    


    <!-- http://www.ejemplo.org/ontologias/turismo#HighQualityRestaurant -->


    <owl:Class rdf:about="http://www.ejemplo.org/ontologias/turismo#HighQualityRestaurant">
        <rdfs:subClassOf rdf:resource="http://www.ejemplo.org/ontologias/turismo#Restaurants"/>
        <rdfs:comment>Represents a restaurant with an average rating higher than 4.5, classified as a high quality restaurant</rdfs:comment>
        <rdfs:label>HighQualityRestaurant</rdfs:label>
    </owl:Class>
    


    <!-- http://www.ejemplo.org/ontologias/turismo#Hotels -->


    <owl:Class rdf:about="http://www.ejemplo.org/ontologias/turismo#Hotels">
        <rdfs:subClassOf rdf:resource="http://www.ejemplo.org/ontologias/turismo#Tourism"/>
        <rdfs:comment>Hotels are commercial establishments that provide lodging, and often meals and other services, for travelers and tourists</rdfs:comment>
        <rdfs:label>Hotels</rdfs:label>
        <owl1:sameAs>https://dbpedia.org/page/Hotel</owl1:sameAs>
    </owl:Class>
    


    <!-- http://www.ejemplo.org/ontologias/turismo#Italian -->


    <owl:Class rdf:about="http://www.ejemplo.org/ontologias/turismo#Italian">
        <rdfs:subClassOf rdf:resource="http://www.ejemplo.org/ontologias/turismo#Restaurants"/>
        <rdfs:comment>Establishments that serve traditional Italian cuisine, characterized by dishes such as pasta, pizza, and risotto, often using fresh ingredients and olive oil</rdfs:comment>
        <rdfs:label>Italian</rdfs:label>
    </owl:Class>
    


    <!-- http://www.ejemplo.org/ontologias/turismo#Japanese -->


    <owl:Class rdf:about="http://www.ejemplo.org/ontologias/turismo#Japanese">
        <rdfs:subClassOf rdf:resource="http://www.ejemplo.org/ontologias/turismo#Restaurants"/>
        <rdfs:comment>Establishments that serve traditional Japanese cuisine such as sushi, ramen, and tempura</rdfs:comment>
        <rdfs:label>Japanese</rdfs:label>
    </owl:Class>
    


    <!-- http://www.ejemplo.org/ontologias/turismo#Luxury -->


    <owl:Class rdf:about="http://www.ejemplo.org/ontologias/turismo#Luxury">
        <rdfs:subClassOf rdf:resource="http://www.ejemplo.org/ontologias/turismo#Hotels"/>
        <rdfs:comment>Hotels that offer high-end services and amenities, providing an upscale and luxurious experience for guests</rdfs:comment>
        <rdfs:label>Luxury</rdfs:label>
    </owl:Class>
    


    <!-- http://www.ejemplo.org/ontologias/turismo#Mediterranean -->


    <owl:Class rdf:about="http://www.ejemplo.org/ontologias/turismo#Mediterranean">
        <rdfs:subClassOf rdf:resource="http://www.ejemplo.org/ontologias/turismo#Restaurants"/>
        <rdfs:comment>Establishments that specialize in Mediterranean cuisine, featuring dishes that emphasize fresh vegetables, olive oil, seafood, and herbs from the Mediterranean region</rdfs:comment>
        <rdfs:label>Mediterranean</rdfs:label>
    </owl:Class>
    


    <!-- http://www.ejemplo.org/ontologias/turismo#Metro -->


    <owl:Class rdf:about="http://www.ejemplo.org/ontologias/turismo#Metro">
        <rdfs:subClassOf rdf:resource="http://www.ejemplo.org/ontologias/turismo#Transports"/>
        <rdfs:comment>Metro is a type of rapid transit system, usually underground, that provides fast and efficient transportation within urban areas</rdfs:comment>
        <rdfs:label>Metro</rdfs:label>
    </owl:Class>
    


    <!-- http://www.ejemplo.org/ontologias/turismo#Mexican -->


    <owl:Class rdf:about="http://www.ejemplo.org/ontologias/turismo#Mexican">
        <rdfs:subClassOf rdf:resource="http://www.ejemplo.org/ontologias/turismo#Restaurants"/>
        <rdfs:comment>Establishments that specialize in traditional Mexican cuisine, often featuring dishes such as tacos, enchiladas, and guacamole</rdfs:comment>
        <rdfs:label>Mexican</rdfs:label>
    </owl:Class>
    


    <!-- http://www.ejemplo.org/ontologias/turismo#Monument -->


    <owl:Class rdf:about="http://www.ejemplo.org/ontologias/turismo#Monument">
        <rdfs:subClassOf rdf:resource="http://www.ejemplo.org/ontologias/turismo#Attractions"/>
        <rdfs:comment>A significant structure or site, often with historical, cultural, or architectural importance, that attracts visitors</rdfs:comment>
        <rdfs:label>Monument</rdfs:label>
    </owl:Class>
    


    <!-- http://www.ejemplo.org/ontologias/turismo#Museum -->


    <owl:Class rdf:about="http://www.ejemplo.org/ontologias/turismo#Museum">
        <rdfs:subClassOf rdf:resource="http://www.ejemplo.org/ontologias/turismo#Attractions"/>
        <rdfs:comment>A place where historical, cultural, or artistic exhibits are displayed for the public to view and learn from</rdfs:comment>
        <rdfs:label>Museum</rdfs:label>
    </owl:Class>
    


    <!-- http://www.ejemplo.org/ontologias/turismo#MusicEvent -->


    <owl:Class rdf:about="http://www.ejemplo.org/ontologias/turismo#MusicEvent">
        <rdfs:subClassOf rdf:resource="http://www.ejemplo.org/ontologias/turismo#Events"/>
        <rdfs:comment>Events centered around music, such as concerts, music festivals, and live performances, featuring various genres and artists</rdfs:comment>
        <rdfs:label>MusicEvent</rdfs:label>
    </owl:Class>
    


    <!-- http://www.ejemplo.org/ontologias/turismo#Restaurants -->


    <owl:Class rdf:about="http://www.ejemplo.org/ontologias/turismo#Restaurants">
        <rdfs:subClassOf rdf:resource="http://www.ejemplo.org/ontologias/turismo#Tourism"/>
        <rdfs:subClassOf>
            <owl:Restriction>
                <owl:onProperty rdf:resource="http://www.ejemplo.org/ontologias/turismo#hasARating"/>
                <owl:qualifiedCardinality rdf:datatype="http://www.w3.org/2001/XMLSchema#nonNegativeInteger">1</owl:qualifiedCardinality>
                <owl:onDataRange rdf:resource="http://www.w3.org/2001/XMLSchema#decimal"/>
            </owl:Restriction>
        </rdfs:subClassOf>
        <rdfs:comment>Restaurants are establishments that prepare and serve food and drinks to customers, often catering to both locals and tourists</rdfs:comment>
        <rdfs:label>Restaurants</rdfs:label>
        <owl1:sameAs>https://dbpedia.org/page/Restaurant</owl1:sameAs>
    </owl:Class>
    


    <!-- http://www.ejemplo.org/ontologias/turismo#Rural -->


    <owl:Class rdf:about="http://www.ejemplo.org/ontologias/turismo#Rural">
        <rdfs:subClassOf rdf:resource="http://www.ejemplo.org/ontologias/turismo#Hotels"/>
        <rdfs:comment>Hotels located in rural or countryside areas, offering a peaceful environment and connection to nature</rdfs:comment>
        <rdfs:label>Rural</rdfs:label>
    </owl:Class>
    


    <!-- http://www.ejemplo.org/ontologias/turismo#Sporting -->


    <owl:Class rdf:about="http://www.ejemplo.org/ontologias/turismo#Sporting">
        <rdfs:subClassOf rdf:resource="http://www.ejemplo.org/ontologias/turismo#Events"/>
        <rdfs:comment>Events focused on physical activities and competitions, such as sports matches, tournaments, and athletic events</rdfs:comment>
        <rdfs:label>Sporting</rdfs:label>
    </owl:Class>
    


    <!-- http://www.ejemplo.org/ontologias/turismo#Taxi -->


    <owl:Class rdf:about="http://www.ejemplo.org/ontologias/turismo#Taxi">
        <rdfs:subClassOf rdf:resource="http://www.ejemplo.org/ontologias/turismo#Transports"/>
        <rdfs:comment>Taxi is a type of transport service that provides on-demand rides for individual passengers or small groups, typically within a city</rdfs:comment>
        <rdfs:label>Taxi</rdfs:label>
    </owl:Class>
    


    <!-- http://www.ejemplo.org/ontologias/turismo#Technology -->


    <owl:Class rdf:about="http://www.ejemplo.org/ontologias/turismo#Technology">
        <rdfs:subClassOf rdf:resource="http://www.ejemplo.org/ontologias/turismo#Events"/>
        <rdfs:comment>Events focused on technological innovations and developments, such as tech conferences, product launches, and exhibitions of new technologies</rdfs:comment>
        <rdfs:label>Technology</rdfs:label>
    </owl:Class>
    


    <!-- http://www.ejemplo.org/ontologias/turismo#Tourism -->


    <owl:Class rdf:about="http://www.ejemplo.org/ontologias/turismo#Tourism">
        <rdfs:comment>Tourism involves travel for leisure, business, or cultural purposes</rdfs:comment>
        <rdfs:label>Tourism</rdfs:label>
    </owl:Class>
    


    <!-- http://www.ejemplo.org/ontologias/turismo#Tourist -->


    <owl:Class rdf:about="http://www.ejemplo.org/ontologias/turismo#Tourist">
        <rdfs:subClassOf rdf:resource="http://www.ejemplo.org/ontologias/turismo#Hotels"/>
        <rdfs:comment>Hotels specifically designed or popular with tourists, offering services and amenities tailored to their needs</rdfs:comment>
        <rdfs:label>Tourist</rdfs:label>
    </owl:Class>
    


    <!-- http://www.ejemplo.org/ontologias/turismo#Tram -->


    <owl:Class rdf:about="http://www.ejemplo.org/ontologias/turismo#Tram">
        <rdfs:subClassOf rdf:resource="http://www.ejemplo.org/ontologias/turismo#Transports"/>
        <rdfs:comment>Tram is a rail-based public transport vehicle that typically operates on tracks laid along urban streets, providing short- to medium-distance service</rdfs:comment>
        <rdfs:label>Tram</rdfs:label>
    </owl:Class>
    


    <!-- http://www.ejemplo.org/ontologias/turismo#Transports -->


    <owl:Class rdf:about="http://www.ejemplo.org/ontologias/turismo#Transports">
        <rdfs:subClassOf rdf:resource="http://www.ejemplo.org/ontologias/turismo#Tourism"/>
        <rdfs:comment>Transports refer to the various means of travel used by tourists to reach and move between destinations, such as buses, trains, airplanes, or rental cars</rdfs:comment>
        <rdfs:label>Transports</rdfs:label>
    </owl:Class>
    


    <!-- 
    ///////////////////////////////////////////////////////////////////////////////////////
    //
    // Individuals
    //
    ///////////////////////////////////////////////////////////////////////////////////////
     -->


    


    <!-- http://example.org/OntologiaTurismo#GeneralMeter -->


    <owl:NamedIndividual rdf:about="http://example.org/OntologiaTurismo#GeneralMeter">
        <rdf:type rdf:resource="http://www.ejemplo.org/ontologias/turismo#Transports"/>
        <rdfs:comment>GeneralMeter</rdfs:comment>
        <rdfs:comment>Subway transportation in cities</rdfs:comment>
    </owl:NamedIndividual>
    


    <!-- http://www.ejemplo.org/ontologias/turismo#AtraccionCastilloZaragoza -->


    <owl:NamedIndividual rdf:about="http://www.ejemplo.org/ontologias/turismo#AtraccionCastilloZaragoza">
        <rdf:type rdf:resource="http://www.ejemplo.org/ontologias/turismo#Monument"/>
        <rdfs:comment>Represents a tourist attraction, a historic castle located in the city of Zaragoza</rdfs:comment>
        <rdfs:label>AtraccionCastilloZaragoza</rdfs:label>
    </owl:NamedIndividual>
    


    <!-- http://www.ejemplo.org/ontologias/turismo#Barcelona -->


    <owl:NamedIndividual rdf:about="http://www.ejemplo.org/ontologias/turismo#Barcelona">
        <rdf:type rdf:resource="http://www.ejemplo.org/ontologias/turismo#Cities"/>
        <turismo:HasTypesOfTransportation rdf:resource="http://example.org/OntologiaTurismo#GeneralMeter"/>
        <rdfs:comment>A major city in northeastern Spain, renowned for its modernist architecture, cultural heritage, and its Mediterranean beaches</rdfs:comment>
        <rdfs:label>Barcelona</rdfs:label>
    </owl:NamedIndividual>
    


    <!-- http://www.ejemplo.org/ontologias/turismo#Bilbao -->


    <owl:NamedIndividual rdf:about="http://www.ejemplo.org/ontologias/turismo#Bilbao">
        <rdf:type rdf:resource="http://www.ejemplo.org/ontologias/turismo#Cities"/>
        <turismo:HasTypesOfTransportation rdf:resource="http://example.org/OntologiaTurismo#GeneralMeter"/>
        <rdfs:comment>A dynamic city in northern Spain, famous for its modern architecture, the Guggenheim Museum, and its rich Basque culture</rdfs:comment>
        <rdfs:label>Bilbao</rdfs:label>
    </owl:NamedIndividual>
    


    <!-- http://www.ejemplo.org/ontologias/turismo#Cadiz -->


    <owl:NamedIndividual rdf:about="http://www.ejemplo.org/ontologias/turismo#Cadiz">
        <rdf:type rdf:resource="http://www.ejemplo.org/ontologias/turismo#Cities"/>
        <turismo:HasTypesOfTransportation rdf:resource="http://example.org/OntologiaTurismo#GeneralMeter"/>
        <rdfs:comment>A port city in southwestern Spain, considered one of the oldest continuously inhabited cities in Western Europe, known for its historic sites and coastal charm</rdfs:comment>
        <rdfs:label>Cadiz</rdfs:label>
        <owl1:sameAs>https://dbpedia.org/page/C%C3%A1diz</owl1:sameAs>
    </owl:NamedIndividual>
    


    <!-- http://www.ejemplo.org/ontologias/turismo#EventoCongresoCadiz -->


    <owl:NamedIndividual rdf:about="http://www.ejemplo.org/ontologias/turismo#EventoCongresoCadiz">
        <rdf:type rdf:resource="http://www.ejemplo.org/ontologias/turismo#Events"/>
        <turismo:HeldIn rdf:resource="http://www.ejemplo.org/ontologias/turismo#Cadiz"/>
        <rdfs:comment>Represents a congress event that takes place in the city of Cádiz</rdfs:comment>
        <rdfs:label>EventoCongresoCadiz</rdfs:label>
    </owl:NamedIndividual>
    


    <!-- http://www.ejemplo.org/ontologias/turismo#HotelVistaSevilla -->


    <owl:NamedIndividual rdf:about="http://www.ejemplo.org/ontologias/turismo#HotelVistaSevilla">
        <rdf:type rdf:resource="http://www.ejemplo.org/ontologias/turismo#Hotels"/>
        <turismo:hasName>Hotel Vista Sevilla</turismo:hasName>
        <rdfs:comment>Represents a hotel located in the city of Seville</rdfs:comment>
        <rdfs:label>HotelVistaSevilla</rdfs:label>
    </owl:NamedIndividual>
    


    <!-- http://www.ejemplo.org/ontologias/turismo#Madrid -->


    <owl:NamedIndividual rdf:about="http://www.ejemplo.org/ontologias/turismo#Madrid">
        <rdf:type rdf:resource="http://www.ejemplo.org/ontologias/turismo#Cities"/>
        <turismo:HasTypesOfTransportation rdf:resource="http://example.org/OntologiaTurismo#GeneralMeter"/>
        <rdfs:comment>The capital city of Spain, known for its historical landmarks, vibrant culture, museums, and as a political and economic center</rdfs:comment>
        <rdfs:label>Madrid</rdfs:label>
    </owl:NamedIndividual>
    


    <!-- http://www.ejemplo.org/ontologias/turismo#Malaga -->


    <owl:NamedIndividual rdf:about="http://www.ejemplo.org/ontologias/turismo#Malaga">
        <rdf:type rdf:resource="http://www.ejemplo.org/ontologias/turismo#Cities"/>
        <turismo:HasTypesOfTransportation rdf:resource="http://example.org/OntologiaTurismo#GeneralMeter"/>
        <rdfs:comment>A vibrant coastal city in southern Spain, known for its Mediterranean beaches, Picasso Museum, and lively cultural scene</rdfs:comment>
        <rdfs:label>Malaga</rdfs:label>
    </owl:NamedIndividual>
    


    <!-- http://www.ejemplo.org/ontologias/turismo#Pamplona -->


    <owl:NamedIndividual rdf:about="http://www.ejemplo.org/ontologias/turismo#Pamplona">
        <rdf:type rdf:resource="http://www.ejemplo.org/ontologias/turismo#Cities"/>
        <turismo:HasTypesOfTransportation rdf:resource="http://example.org/OntologiaTurismo#GeneralMeter"/>
        <rdfs:comment>A city in northern Spain, internationally known for the Running of the Bulls during the San Fermín festival</rdfs:comment>
        <rdfs:label>Pamplona</rdfs:label>
    </owl:NamedIndividual>
    


    <!-- http://www.ejemplo.org/ontologias/turismo#RestauranteTradicionToledo -->


    <owl:NamedIndividual rdf:about="http://www.ejemplo.org/ontologias/turismo#RestauranteTradicionToledo">
        <rdf:type rdf:resource="http://www.ejemplo.org/ontologias/turismo#Restaurants"/>
        <turismo:hasARating rdf:datatype="http://www.w3.org/2001/XMLSchema#decimal">4.5</turismo:hasARating>
        <rdfs:comment>Represents a traditional restaurant located in the city of Toledo</rdfs:comment>
        <rdfs:label>RestauranteTradicionToledo</rdfs:label>
    </owl:NamedIndividual>
    


    <!-- http://www.ejemplo.org/ontologias/turismo#SanSebastian -->


    <owl:NamedIndividual rdf:about="http://www.ejemplo.org/ontologias/turismo#SanSebastian">
        <rdf:type rdf:resource="http://www.ejemplo.org/ontologias/turismo#Cities"/>
        <turismo:HasTypesOfTransportation rdf:resource="http://example.org/OntologiaTurismo#GeneralMeter"/>
        <rdfs:comment>A coastal city in northern Spain, famous for its beautiful beaches, Basque cuisine, and the annual San Sebastián International Film Festival</rdfs:comment>
        <rdfs:label>SanSebastian</rdfs:label>
    </owl:NamedIndividual>
    


    <!-- http://www.ejemplo.org/ontologias/turismo#Sevilla -->


    <owl:NamedIndividual rdf:about="http://www.ejemplo.org/ontologias/turismo#Sevilla">
        <rdf:type rdf:resource="http://www.ejemplo.org/ontologias/turismo#Cities"/>
        <turismo:HasTypesOfTransportation rdf:resource="http://example.org/OntologiaTurismo#GeneralMeter"/>
        <rdfs:comment>A historic city in southern Spain, renowned for its flamenco culture, Moorish architecture, and landmarks such as the Seville Cathedral and the Alcázar</rdfs:comment>
        <rdfs:label>Sevilla</rdfs:label>
    </owl:NamedIndividual>
    


    <!-- http://www.ejemplo.org/ontologias/turismo#Toledo -->


    <owl:NamedIndividual rdf:about="http://www.ejemplo.org/ontologias/turismo#Toledo">
        <rdf:type rdf:resource="http://www.ejemplo.org/ontologias/turismo#Cities"/>
        <turismo:HasTypesOfTransportation rdf:resource="http://example.org/OntologiaTurismo#GeneralMeter"/>
        <rdfs:comment>A historic city in central Spain, known for its medieval architecture, rich cultural heritage, and significance in Spanish history</rdfs:comment>
        <rdfs:label>Toledo</rdfs:label>
    </owl:NamedIndividual>
    


    <!-- http://www.ejemplo.org/ontologias/turismo#Valencia -->


    <owl:NamedIndividual rdf:about="http://www.ejemplo.org/ontologias/turismo#Valencia">
        <rdf:type rdf:resource="http://www.ejemplo.org/ontologias/turismo#Cities"/>
        <turismo:HasTypesOfTransportation rdf:resource="http://example.org/OntologiaTurismo#GeneralMeter"/>
        <rdfs:comment>A vibrant city on Spain&apos;s southeastern coast, famous for its arts, science complex, beaches, and the annual Las Fallas festival</rdfs:comment>
        <rdfs:label>Valencia</rdfs:label>
    </owl:NamedIndividual>
    


    <!-- http://www.ejemplo.org/ontologias/turismo#Zaragoza -->


    <owl:NamedIndividual rdf:about="http://www.ejemplo.org/ontologias/turismo#Zaragoza">
        <rdf:type rdf:resource="http://www.ejemplo.org/ontologias/turismo#Cities"/>
        <turismo:HasTypesOfTransportation rdf:resource="http://example.org/OntologiaTurismo#GeneralMeter"/>
        <rdfs:comment>A historic city in northeastern Spain, known for its Roman and Moorish architecture, the Basilica del Pilar, and its vibrant cultural scene</rdfs:comment>
        <rdfs:label>Zaragoza</rdfs:label>
    </owl:NamedIndividual>
    


    <!-- 
    ///////////////////////////////////////////////////////////////////////////////////////
    //
    // Rules
    //
    ///////////////////////////////////////////////////////////////////////////////////////
     -->


    <rdf:Description rdf:about="http://www.semanticweb.org/alfbe/ontologies/2025/3/untitled-ontology-13/c">
        <rdf:type rdf:resource="http://www.w3.org/2003/11/swrl#Variable"/>
    </rdf:Description>
    <rdf:Description rdf:about="http://www.semanticweb.org/alfbe/ontologies/2025/3/untitled-ontology-13/t">
        <rdf:type rdf:resource="http://www.w3.org/2003/11/swrl#Variable"/>
    </rdf:Description>
    <rdf:Description rdf:about="http://www.semanticweb.org/alfbe/ontologies/2025/3/untitled-ontology-13/e">
        <rdf:type rdf:resource="http://www.w3.org/2003/11/swrl#Variable"/>
    </rdf:Description>
    <rdf:Description>
        <swrla:isRuleEnabled rdf:datatype="http://www.w3.org/2001/XMLSchema#boolean">true</swrla:isRuleEnabled>
        <rdfs:comment>If a city has cultural events then it is considered a cultural city</rdfs:comment>
        <rdfs:label>CulturalCityR3</rdfs:label>
        <rdf:type rdf:resource="http://www.w3.org/2003/11/swrl#Imp"/>
        <swrl:body>
            <rdf:Description>
                <rdf:type rdf:resource="http://www.w3.org/2003/11/swrl#AtomList"/>
                <rdf:first>
                    <rdf:Description>
                        <rdf:type rdf:resource="http://www.w3.org/2003/11/swrl#ClassAtom"/>
                        <swrl:classPredicate rdf:resource="http://www.ejemplo.org/ontologias/turismo#CulturalEvent"/>
                        <swrl:argument1 rdf:resource="http://www.semanticweb.org/alfbe/ontologies/2025/3/untitled-ontology-13/e"/>
                    </rdf:Description>
                </rdf:first>
                <rdf:rest>
                    <rdf:Description>
                        <rdf:type rdf:resource="http://www.w3.org/2003/11/swrl#AtomList"/>
                        <rdf:first>
                            <rdf:Description>
                                <rdf:type rdf:resource="http://www.w3.org/2003/11/swrl#IndividualPropertyAtom"/>
                                <swrl:propertyPredicate rdf:resource="http://www.ejemplo.org/ontologias/turismo#HeldIn"/>
                                <swrl:argument1 rdf:resource="http://www.semanticweb.org/alfbe/ontologies/2025/3/untitled-ontology-13/e"/>
                                <swrl:argument2 rdf:resource="http://www.semanticweb.org/alfbe/ontologies/2025/3/untitled-ontology-13/c"/>
                            </rdf:Description>
                        </rdf:first>
                        <rdf:rest rdf:resource="http://www.w3.org/1999/02/22-rdf-syntax-ns#nil"/>
                    </rdf:Description>
                </rdf:rest>
            </rdf:Description>
        </swrl:body>
        <swrl:head>
            <rdf:Description>
                <rdf:type rdf:resource="http://www.w3.org/2003/11/swrl#AtomList"/>
                <rdf:first>
                    <rdf:Description>
                        <rdf:type rdf:resource="http://www.w3.org/2003/11/swrl#ClassAtom"/>
                        <swrl:classPredicate rdf:resource="http://www.ejemplo.org/ontologias/turismo#CulturalCity"/>
                        <swrl:argument1 rdf:resource="http://www.semanticweb.org/alfbe/ontologies/2025/3/untitled-ontology-13/c"/>
                    </rdf:Description>
                </rdf:first>
                <rdf:rest rdf:resource="http://www.w3.org/1999/02/22-rdf-syntax-ns#nil"/>
            </rdf:Description>
        </swrl:head>
    </rdf:Description>
    <rdf:Description>
        <swrla:isRuleEnabled rdf:datatype="http://www.w3.org/2001/XMLSchema#boolean">true</swrla:isRuleEnabled>
        <rdfs:comment>If an event is held in a city, then the city is classified as a &quot;City with Events&quot;</rdfs:comment>
        <rdfs:label>CityEventR1</rdfs:label>
        <rdf:type rdf:resource="http://www.w3.org/2003/11/swrl#Imp"/>
        <swrl:body>
            <rdf:Description>
                <rdf:type rdf:resource="http://www.w3.org/2003/11/swrl#AtomList"/>
                <rdf:first>
                    <rdf:Description>
                        <rdf:type rdf:resource="http://www.w3.org/2003/11/swrl#ClassAtom"/>
                        <swrl:classPredicate rdf:resource="http://www.ejemplo.org/ontologias/turismo#Events"/>
                        <swrl:argument1 rdf:resource="http://www.semanticweb.org/alfbe/ontologies/2025/3/untitled-ontology-13/e"/>
                    </rdf:Description>
                </rdf:first>
                <rdf:rest>
                    <rdf:Description>
                        <rdf:type rdf:resource="http://www.w3.org/2003/11/swrl#AtomList"/>
                        <rdf:first>
                            <rdf:Description>
                                <rdf:type rdf:resource="http://www.w3.org/2003/11/swrl#IndividualPropertyAtom"/>
                                <swrl:propertyPredicate rdf:resource="http://www.ejemplo.org/ontologias/turismo#HeldIn"/>
                                <swrl:argument1 rdf:resource="http://www.semanticweb.org/alfbe/ontologies/2025/3/untitled-ontology-13/e"/>
                                <swrl:argument2 rdf:resource="http://www.semanticweb.org/alfbe/ontologies/2025/3/untitled-ontology-13/c"/>
                            </rdf:Description>
                        </rdf:first>
                        <rdf:rest rdf:resource="http://www.w3.org/1999/02/22-rdf-syntax-ns#nil"/>
                    </rdf:Description>
                </rdf:rest>
            </rdf:Description>
        </swrl:body>
        <swrl:head>
            <rdf:Description>
                <rdf:type rdf:resource="http://www.w3.org/2003/11/swrl#AtomList"/>
                <rdf:first>
                    <rdf:Description>
                        <rdf:type rdf:resource="http://www.w3.org/2003/11/swrl#ClassAtom"/>
                        <swrl:classPredicate rdf:resource="http://www.ejemplo.org/ontologias/turismo#CityWithEvents"/>
                        <swrl:argument1 rdf:resource="http://www.semanticweb.org/alfbe/ontologies/2025/3/untitled-ontology-13/c"/>
                    </rdf:Description>
                </rdf:first>
                <rdf:rest rdf:resource="http://www.w3.org/1999/02/22-rdf-syntax-ns#nil"/>
            </rdf:Description>
        </swrl:head>
    </rdf:Description>
    <rdf:Description>
        <swrla:isRuleEnabled rdf:datatype="http://www.w3.org/2001/XMLSchema#boolean">true</swrla:isRuleEnabled>
        <rdfs:comment>If a city has metro transportation, it is classified as a Big City</rdfs:comment>
        <rdfs:label>BigCityByMetroR2</rdfs:label>
        <rdf:type rdf:resource="http://www.w3.org/2003/11/swrl#Imp"/>
        <swrl:body>
            <rdf:Description>
                <rdf:type rdf:resource="http://www.w3.org/2003/11/swrl#AtomList"/>
                <rdf:first>
                    <rdf:Description>
                        <rdf:type rdf:resource="http://www.w3.org/2003/11/swrl#ClassAtom"/>
                        <swrl:classPredicate rdf:resource="http://www.ejemplo.org/ontologias/turismo#Cities"/>
                        <swrl:argument1 rdf:resource="http://www.semanticweb.org/alfbe/ontologies/2025/3/untitled-ontology-13/c"/>
                    </rdf:Description>
                </rdf:first>
                <rdf:rest>
                    <rdf:Description>
                        <rdf:type rdf:resource="http://www.w3.org/2003/11/swrl#AtomList"/>
                        <rdf:first>
                            <rdf:Description>
                                <rdf:type rdf:resource="http://www.w3.org/2003/11/swrl#IndividualPropertyAtom"/>
                                <swrl:propertyPredicate rdf:resource="http://www.ejemplo.org/ontologias/turismo#HasTypesOfTransportation"/>
                                <swrl:argument1 rdf:resource="http://www.semanticweb.org/alfbe/ontologies/2025/3/untitled-ontology-13/c"/>
                                <swrl:argument2 rdf:resource="http://www.semanticweb.org/alfbe/ontologies/2025/3/untitled-ontology-13/t"/>
                            </rdf:Description>
                        </rdf:first>
                        <rdf:rest>
                            <rdf:Description>
                                <rdf:type rdf:resource="http://www.w3.org/2003/11/swrl#AtomList"/>
                                <rdf:first>
                                    <rdf:Description>
                                        <rdf:type rdf:resource="http://www.w3.org/2003/11/swrl#ClassAtom"/>
                                        <swrl:classPredicate rdf:resource="http://www.ejemplo.org/ontologias/turismo#Metro"/>
                                        <swrl:argument1 rdf:resource="http://www.semanticweb.org/alfbe/ontologies/2025/3/untitled-ontology-13/t"/>
                                    </rdf:Description>
                                </rdf:first>
                                <rdf:rest rdf:resource="http://www.w3.org/1999/02/22-rdf-syntax-ns#nil"/>
                            </rdf:Description>
                        </rdf:rest>
                    </rdf:Description>
                </rdf:rest>
            </rdf:Description>
        </swrl:body>
        <swrl:head>
            <rdf:Description>
                <rdf:type rdf:resource="http://www.w3.org/2003/11/swrl#AtomList"/>
                <rdf:first>
                    <rdf:Description>
                        <rdf:type rdf:resource="http://www.w3.org/2003/11/swrl#ClassAtom"/>
                        <swrl:classPredicate rdf:resource="http://www.ejemplo.org/ontologias/turismo#BigCity"/>
                        <swrl:argument1 rdf:resource="http://www.semanticweb.org/alfbe/ontologies/2025/3/untitled-ontology-13/c"/>
                    </rdf:Description>
                </rdf:first>
                <rdf:rest rdf:resource="http://www.w3.org/1999/02/22-rdf-syntax-ns#nil"/>
            </rdf:Description>
        </swrl:head>
    </rdf:Description>
</rdf:RDF>



<!-- Generated by the OWL API (version 5.1.18) https://github.com/owlcs/owlapi/ -->


